refinedVST/typing/constrained.v
@@ -42,22 +42,22 @@ Section own_constrained.
   Qed.
   *)
   
-  Global Instance constrained_defined cty P `{!OwnConstraint P} ty `{!DefinedTy cty ty} : DefinedTy cty (own_constrained P ty).
+  Global Instance constrained_defined P `{!OwnConstraint P} ty `{!DefinedTy ty} : DefinedTy (own_constrained P ty).
   Proof.
-    iIntros (?) "(? & _)".
+    iIntros (??) "(? & _)".
     by iApply defined_ty.
   Qed.
 
-  Lemma copy_as_own_constrained l β cty P `{!OwnConstraint P} ty {HC: CopyAs l β cty ty} T:
-    (P β -∗ (HC T).(i2p_P)) ⊢ copy_as l β cty (own_constrained P ty) T.
+  Lemma copy_as_own_constrained l β P `{!OwnConstraint P} ty {HC: CopyAs l β ty} T:
+    (P β -∗ (HC T).(i2p_P)) ⊢ copy_as l β (own_constrained P ty) T.
   Proof.
     iIntros "HT [Hty HP]". iDestruct (i2p_proof with "(HT HP)") as "HT". by iApply "HT".
   Qed.
   Definition copy_as_own_constrained_inst := [instance copy_as_own_constrained].
   Global Existing Instance copy_as_own_constrained_inst.
 
-  Lemma copy_as_defined_own_constrained l β cty P `{!OwnConstraint P} ty {HC: CopyAsDefined l β cty ty} T:
-    (P β -∗ (HC T).(i2p_P)) ⊢ copy_as_defined l β cty (own_constrained P ty) T.
+  Lemma copy_as_defined_own_constrained l β P `{!OwnConstraint P} ty {HC: CopyAsDefined l β ty} T:
+    (P β -∗ (HC T).(i2p_P)) ⊢ copy_as_defined l β (own_constrained P ty) T.
   Proof.
     iIntros "HT [Hty HP]". iDestruct (i2p_proof with "(HT HP)") as "HT". by iApply "HT".
   Qed.
